@prefix : <http://open-multinet.info/ontology/omn-lifecycle#> .
@prefix dc: <http://purl.org/dc/elements/1.1/> .
@prefix owl: <http://www.w3.org/2002/07/owl#> .
@prefix rdf: <http://www.w3.org/1999/02/22-rdf-syntax-ns#> .
@prefix xml: <http://www.w3.org/XML/1998/namespace> .
@prefix xsd: <http://www.w3.org/2001/XMLSchema#> .
@prefix rdfs: <http://www.w3.org/2000/01/rdf-schema#> .
@prefix dcterms: <http://purl.org/dc/terms/> .
@base <http://open-multinet.info/ontology/omn-lifecycle> .

<http://open-multinet.info/ontology/omn-template> rdf:type owl:Ontology ;
                                         
                                         rdfs:label "omn"@en ;
                                         
                                         dc:date "2014-11-27"^^xsd:date ;
                                         
                                         owl:versionInfo "2014-11-27"^^xsd:string ;
                                         
                                         dc:title "Open-Multinet Upper Ontology"^^xsd:string ;
                                         
                                         dc:description "This ontology defines generic concepts related to different types of lifecycle."^^xsd:string ;
                                         
                                         dc:publisher <http://open-multinet.org> ;
                                         
                                         dcterms:license <http://creativecommons.org/licenses/by/4.0/> .


#################################################################
#
#    Object Properties
#
#################################################################




				


#################################################################
#
#    Data properties
#
#################################################################




#################################################################
#
#    Classes
#
#################################################################


# Name	Description	Example	Parent	See also
# State	The current state of the resource		omn:Attribute	
# Offering	A collection (group) of services and resources provided by an Infrastructure. The collection is the result of the application of Policies.		omn:Group	SFA ListResources
# Request	A collection (group) of resources/services/groups requested by the user		omn:Group	
# Confirmation	A collection (group) of resources/services/groups  confirmed to be allocated for the user.		omn:Group	
# Manifest	A collection (group) of resources/services/groups  allocated for the user.		omn:Group	



###  http://open-multinet.info/ontology/omn-lifecycle#State

:State 		rdf:type owl:Class ;

			rdfs:comment "The current state of the resource"@en ;
         
         	rdfs:subClassOf :Attribute .



###  http://open-multinet.info/ontology/omn-lifecycle#Offering

:Offering 	rdf:type owl:Class ;

			rdfs:comment "A collection (group) of services and resources provided by an Infrastructure. The collection is the result of the application of Policies."@en ;

			# rdfs:seeAlso sfa:ListResources ;
          
          	rdfs:subClassOf :Group .



###  http://open-multinet.info/ontology/omn-lifecycle#Request

:Request 	rdf:type owl:Class ;
	
			rdfs:comment "A collection (group) of resources/services/groups requested by the user"@en ;
         
         	rdfs:subClassOf :Group .




###  http://open-multinet.info/ontology/omn-lifecycle#Confirmation

:Confirmation 	rdf:type owl:Class ;

			rdfs:comment "A collection (group) of resources/services/groups confirmed to be allocated for the user."@en ;
         
         	rdfs:subClassOf :Group .



###  http://open-multinet.info/ontology/omn-lifecycle#Manifest

:Manifest 	rdf:type owl:Class ;

			rdfs:comment "A collection (group) of resources/services/groups allocated for the user."@en ;
         
         	rdfs:subClassOf :Group .




###  Generated by the OWL API (version 3.5.0) http://owlapi.sourceforge.net

